example proofs for inner conflict in then

example_small_examples.thy
@@ -94,4 +94,58 @@ lemma many_this_char_no_peek_past_any_other_char:
   using many_char_for_predicate_does_not_consume_past_char3[of _ \<open>C'\<close>]
   by blast
 
+
+lemma induct_on_printed_value_example:
+  assumes hra: "has_result (parse A) i a []"
+  assumes prb: "p_has_result (print (b_then B C)) b_c pr"
+  shows "has_result (parse A) (i@pr) a pr"
+  apply (insert hra prb)
+  apply (cases pr; clarsimp)
+  subgoal for pr' prs
+    
+    sorry
+  oops
+
+\<comment> \<open>Empty list case\<close>
+definition "empty_list = b_then (char_ws CHR ''['') (ws_char CHR '']'')"
+
+lemma empty_list_no_peek_past_end:
+  "does_not_peek_past_end (parse empty_list)"
+  unfolding empty_list_def
+  apply (rule then_does_not_peek_past_end_with_inner_conflict)
+  subgoal by pasi_pngi
+  subgoal by pasi_pngi
+  subgoal for c1 c2 a l b l'
+    by (rule exI[of _ \<open>c2@l'\<close>]; auto simp add: NER_simps split: list.splits)
+  done
+
+lemma empty_list_wf:
+  "bidef_well_formed empty_list"
+  unfolding empty_list_def
+  apply (rule b_then_well_formed)
+  subgoal by (clarsimp simp add: char_ws_well_formed)
+  subgoal by (clarsimp simp add: ws_char_well_formed)  
+  unfolding pa_does_not_eat_into_pb_nondep_def
+  by (clarsimp simp add: fp_NER NER_simps)
+
+lemma empty_list_example_proof:
+  assumes hr1: "has_result (parse (char_ws CHR ''['')) c1 () []"
+  assumes hr2: "has_result (parse (ws_char CHR '']'')) c2 () []"
+  shows "has_result (parse empty_list) (c1@c2) ((), ()) []"
+  apply (insert hr1 hr2; clarsimp simp add: empty_list_def)
+  apply (clarsimp simp add: b_then_has_result b_then_p_has_result)
+  apply (rule exI[of _ \<open>dropWhile (\<lambda>c. c \<in> whitespace_chars) (tl c1@c2)\<close>]; auto)
+  subgoal
+    apply (auto simp add: NER_simps split: list.splits)
+    apply (rule exI[of _ \<open>tl c1 @ (butlast c2)\<close>]; auto)
+    subgoal by (metis snoc_eq_iff_butlast takeWhile_dropWhile_id)
+    subgoal
+      apply (cases c2; clarsimp split: if_splits)
+      by (smt (verit, best) dropWhile_append dropWhile_eq_Nil_conv self_append_conv2 snoc_eq_iff_butlast takeWhile_dropWhile_id)
+    done
+  subgoal by (auto simp add: NER_simps)
+  done
+
+thm print_empty
+
 end
